\documentclass{article}
\usepackage{times}
\usepackage{setspace}
\usepackage{lineno}
\usepackage{amsmath}
\linenumbers
\doublespacing

\begin{document}

\begin{align}
& \mathrm{E}[A_{\mathrm{area} \, i}]
= \alpha_0\mathrm{LMAm}_{i}^{\alpha_m}\mathrm{LMAs}_i^{\alpha_s}  =  \alpha_0 (f_i \mathrm{LMA}_{i})^{\alpha_m} \bigl\{(1-f_i) \mathrm{LMA}_{i}\bigr\}^{\alpha_s} (\#eq:E-A) \\
& \mathrm{E}[\mathrm{LL_i}] = \beta_0\mathrm{LMAm}_{i}^{\beta_m} \mathrm{LMAs}_{i}^{\beta_s}   = \beta_0 (f_i \mathrm{LMA}_{i})^{\beta_m} \bigl\{(1-f_i) \mathrm{LMA}_{i}\bigr\}^{\beta_s} (\#eq:E-LL) \\
& \mathrm{E}[R_{\mathrm{area} \, i}]
= \gamma_0\mathrm{LMAm}_{i}^{\gamma_m}Ä± \mathrm{LMAs}_{i}^{\gamma_s}
= \gamma_0 (f_i \mathrm{LMA}_{i})^{\gamma_m}  \bigl\{(1-f_i)\mathrm{LMA}_{i}\bigr\}^{\gamma_s} (\#eq:E-R)
\end{align}

\begin{align}
Z =
\left(
\begin{array}{rrr}
\alpha_0 &\beta_0 &\gamma_0 \\
\alpha_m &\beta_m &\gamma_m \\
\alpha_s &\beta_s &\gamma_s
\end{array}
\right)
\end{align}

\begin{align}
\left(
\begin{array}{ccc}
\mathrm{ln}[A_{\mathrm{area} \, i}]\\
\mathrm{ln}[\mathrm{LL}_i]\\
\mathrm{ln}[R_{\mathrm{area} \, i}]
\end{array}
\right)
\sim \mathrm{MVN}
\left(
\begin{array}{rrr}
\mu_{1i} &\\
\mu_{2i} &\boldsymbol{\\Sigma}\\
\mu_{3i} &
\end{array}
\right) (\#eq:MVN)
\end{align}

\begin{align}
\mathrm{Var}(Y = X1 + X2) = \mathrm{Var}(X1) + \mathrm{Var}(X2) + 2 \mathrm{Cov}(X1,X2) (\#eq:var)
\end{align}

\begin{align}
\mathrm{E[LL]}_i = \beta_0\mathrm{LMAm}_{i}^{\beta_m} \mathrm{LMAs}_{i}^{\beta_s} exp(\theta Light_i) (\#eq:E-LL2)
\end{align}

\begin{align}
A_{\mathrm{area} \, i} = a (LMA_i)^{b}\epsilon_i (\#eq:mass)
\end{align}


\begin{align}
\mu_{1i} = \mathrm{ln}\alpha_0
+ \alpha_m \mathrm{ln}f_i
+ \alpha_s \mathrm{ln}(1-f_i)
+ \mathrm{ln}(\alpha_m + \alpha_s) (\#eq:mu1)\\
\mu_{2i} = \mathrm{ln}\beta_0
+ \beta_m \mathrm{ln}f_i
+ \beta_s \mathrm{ln}(1-f_i)
+ \mathrm{ln}(\beta_m + \beta_s) (\#eq:mu3)\\
\mu_{3i} = \mathrm{ln}\gamma_0
+ \gamma_m \mathrm{ln}f_i
+ \gamma_s \mathrm{ln}(1-f_i)
+ \mathrm{ln}(\gamma_m + \gamma_s) (\#eq:mu3)
\end{align}

\begin{align}
\boldsymbol{\Sigma} =
\left(
\begin{array}{ccc}
\sigma_1^2 &\rho_{12}\sigma_1\sigma_2 &\rho_{13}\sigma_1\sigma_3 \\
\rho_{12}\sigma_1\sigma_2&\sigma_2^2 &\rho_{23}\sigma_2\sigma_3 \\
\rho_{13}\sigma_1\sigma_3&\rho_{23}\sigma_2\sigma_3 &\sigma_3^2
\end{array}
\right) (\#eq:Sigma)
\end{align}



\begin{align}
\mathrm{Var}(Y = X1 + X2) = \mathrm{Cov}(Y, X1+X2) = \mathrm{Cov}(Y,X1) + \mathrm{Cov}(Y,X2) (#eq:var)
\end{align}


\begin{align}

& A_{\mathrm{area} \; i}
= \alpha_0\mathrm{LMAm}_{i}^{\alpha_m} \epsilon_{1i} =  \alpha_0 f_i \mathrm{LMA}_{i}^{\alpha_m} \epsilon_{1i}\\

& \mathrm{LL_i} = \beta_0\mathrm{LMAs}_{i}^{\beta_s} \epsilon_{2i}  = \beta_0 (1 - f_i)\mathrm{LMAs}_{i}^{\beta_s} \epsilon_{2i}\\

& R_{\mathrm{area} \; i}
= \gamma_0\mathrm{LMAm}_{i}^{\gamma_m} \mathrm{LMAs}_{i}^{\gamma_s} \epsilon_{3i}
= \gamma_0 f_i \mathrm{LMA}_{i}^{\gamma_m}  (1-f_i)\mathrm{LMA}_{i}^{\gamma_s} \epsilon_{3i}\\
\end{align}


\begin{align}

& A_{\mathrm{area} \; i}
= \alpha_0\mathrm{LMAm}_{i}^{\alpha_m} \epsilon_{1i}\\

& \mathrm{LL_i} = \beta_0 A_{\mathrm{area} \; i}^{\beta_m} \mathrm{LMAs}_{i}^{\beta_s} \epsilon_{2i}\\

& R_{\mathrm{area} \; i}
= \gamma_0\mathrm{LMAm}_{i}^{\gamma_m}\mathrm{LMAs}_{i}^{\gamma_s} \epsilon_{3i}\\
\end{align}


\begin{align}
  
& A_{\mathrm{area} \; i}
= \alpha_0\mathrm{LMAm}_{i}^{\alpha_m} (\mathrm{LMAs}_{i}/ \mathrm{LT}_{i})^{\alpha_s}\epsilon_{1i}\\

& \mathrm{LL_i} = \beta_0 A_{\mathrm{area} \; i}^{\beta_m} ({\mathrm{LMAs}_{i}/\mathrm{LT}_{i}})^{\beta_s} \epsilon_{2i}\\

& R_{\mathrm{area} \; i}
= \gamma_0\mathrm{LMAm}_{i}^{\gamma_m} \mathrm{LMAs}_{i}^{\gamma_s} \epsilon_{3i}\\
\end{align}

\end{document}
